Hopcroft_Karp/Ford_Fulkerson_Tbd.thy
@@ -1,0 +1,242 @@
+theory Ford_Fulkerson_Tbd
+  imports
+    "../../matching/Blossom_Algo"
+    Ford_Fulkerson
+begin
+
+text \<open>This theory connects @{term ford_fulkerson.loop'} to @{term find_max_match.find_max_matching}\<close>
+
+section \<open>Convenience lemmas\<close>
+
+lemma edges_of_path_conv:
+  shows "Graph.edges_of_path l = edges_of_path l"
+  by (induct l rule: edges_of_path.induct) simp+
+
+lemma symmetric_diff_conv:
+  shows "Berge2.symmetric_diff = symmetric_diff"
+  unfolding Berge2.symmetric_diff_def symmetric_diff_def
+  ..
+
+lemma matching_conv:
+  shows "Berge2.matching = matching"
+  unfolding Berge2.matching_def matching_def
+  ..
+
+section \<open>Definitions\<close>
+
+definition (in ford_fulkerson) f' :: "'a \<times> 'a \<Rightarrow> 'm \<Rightarrow> 'm" where
+  "f' p \<equiv> M_update (fst p) (snd p)"
+
+definition (in ford_fulkerson) M_tbd_inv :: "'a set set \<Rightarrow> 'm" where
+  "M_tbd_inv M \<equiv> Finite_Set.fold f' M_empty (graph.dEs M)"
+
+definition (in ford_fulkerson) search_aug_path :: "'n \<Rightarrow> 's \<Rightarrow> 's \<Rightarrow> 'a \<Rightarrow> 'a \<Rightarrow> 'm \<Rightarrow> 'a list option" where
+  "search_aug_path G U V s t M \<equiv>
+   if done_1 U V M then None
+   else if done_2 t (m_tbd G U V s t M) then None
+        else Some (p_tbd G U V s t M)"
+
+abbreviation (in ford_fulkerson_valid_input_2) search_aug_path' :: "'a set set \<Rightarrow> 'a set set \<Rightarrow> 'a list option" where
+  "search_aug_path' _ M \<equiv> search_aug_path G U V s t (M_tbd_inv M)"
+
+section \<open>Basic lemmas\<close>
+
+context ford_fulkerson_valid_input_2
+begin
+sublocale find_max_match search_aug_path' "G.E G"
+proof (standard, goal_cases)
+  case (1 M)
+  then show ?case sorry
+next
+  case (2 M p)
+  then show ?case sorry
+next
+  case 3
+  then show ?case sorry
+next
+  case 4
+  then show ?case sorry
+qed
+end
+
+find_theorems "Finite_Set.fold _ _ (set _) = fold _ _ _"
+
+lemma (in ford_fulkerson) lookup_conv:
+  shows "M_lookup (M_tbd_inv (M_tbd M)) = M_lookup M"
+  sorry
+
+lemma (in ford_fulkerson_invar) done_1_conv:
+  shows "done_1 U V (M_tbd_inv (M_tbd M)) = done_1 U V M"
+  sorry
+
+lemma (in ford_fulkerson_invar) done_2_conv:
+  shows "done_2 t (m_tbd G U V s t (M_tbd_inv (M_tbd M))) = done_2 t (m_tbd G U V s t M)"
+  sorry
+
+lemma (in ford_fulkerson_invar) p_tbd_conv:
+  shows "p_tbd G U V s t (M_tbd_inv (M_tbd M)) = p_tbd G U V s t M"
+  sorry
+
+lemma (in ford_fulkerson_invar) find_max_matching_psimps:
+  shows
+    "find_max_matching (M_tbd M) =
+     (if done_1 U V M then (M_tbd M)
+      else if done_2 t (m_tbd G U V s t M) then (M_tbd M)
+           else find_max_matching (M_tbd (augment M (p_tbd G U V s t M))))"
+proof -
+  have find_max_matching_psimps:
+    "find_max_matching (M_tbd M) =
+     (case search_aug_path' (G.E G) (M_tbd M) of
+        None \<Rightarrow> M_tbd M |
+        Some p \<Rightarrow> find_max_matching (symmetric_diff (M_tbd M) (P_tbd p)))"
+  proof -
+    have
+      "find_max_matching (M_tbd M) = 
+       (if \<exists>p. search_aug_path' (G.E G) (M_tbd M) = Some p
+        then find_max_matching (Berge2.symmetric_diff (M_tbd M) (set (Graph.edges_of_path (the (search_aug_path' (G.E G) (M_tbd M))))))
+        else M_tbd M)"
+    using graph_matching_M_tbd finite_M_tbd
+    by (intro find_max_matching_dom find_max_matching.psimps) (simp_all add: matching_conv)
+    hence
+      "find_max_matching (M_tbd M) = 
+       (if \<exists>p. search_aug_path' (G.E G) (M_tbd M) = Some p
+        then find_max_matching (symmetric_diff (M_tbd M) (set (edges_of_path (the (search_aug_path' (G.E G) (M_tbd M))))))
+        else M_tbd M)"
+      by (simp add: symmetric_diff_conv edges_of_path_conv)
+    thus ?thesis
+      by force
+  qed
+  show ?thesis
+  proof (cases "done_1 U V M")
+    case True
+    hence "done_1 U V (M_tbd_inv (M_tbd M))"
+      by (simp add: done_1_conv)
+    hence "search_aug_path' _ (M_tbd M) = None"
+      by (simp add: search_aug_path_def)
+    thus ?thesis
+      using True
+      by (simp add: find_max_matching_psimps)
+  next
+    case not_done_1: False
+    show ?thesis
+    proof (cases "done_2 t (m_tbd G U V s t M)")
+      case True
+      hence "done_2 t (m_tbd G U V s t (M_tbd_inv (M_tbd M)))"
+        by (simp add: done_2_conv)
+      hence "search_aug_path' _ (M_tbd M) = None"
+        by (simp add: search_aug_path_def)
+      thus ?thesis
+        using True
+        by (simp add: find_max_matching_psimps)
+    next
+      case False
+      hence ford_fulkerson_invar_not_done_2: "ford_fulkerson_invar_not_done_2'' M"
+        using ford_fulkerson_invar_axioms not_done_1 False
+        by (intro ford_fulkerson_invar_not_done_2I_2)
+
+      have
+        "\<not> done_1 U V (M_tbd_inv (M_tbd M))"
+        "\<not> done_2 t (m_tbd G U V s t (M_tbd_inv (M_tbd M)))"
+        using not_done_1 False
+        by (simp_all add: done_1_conv done_2_conv)
+      hence "search_aug_path' _ (M_tbd M) = Some (p_tbd G U V s t (M_tbd_inv (M_tbd M)))"
+        by (simp add: search_aug_path_def)
+      hence
+        "find_max_matching (M_tbd M) =
+         find_max_matching (symmetric_diff (M_tbd M) (P_tbd (p_tbd G U V s t (M_tbd_inv (M_tbd M)))))"
+        using not_done_1 False
+        by (simp add: find_max_matching_psimps)
+      thus ?thesis
+        unfolding p_tbd_conv
+        using not_done_1 False
+        using invar_M symmetric_M
+        using ford_fulkerson_invar_not_done_2.augmenting_path_p_tbd[OF ford_fulkerson_invar_not_done_2]
+        using ford_fulkerson_invar_not_done_2.distinct_p_tbd[OF ford_fulkerson_invar_not_done_2]
+        using ford_fulkerson_invar_not_done_2.even_length_p_tbd[OF ford_fulkerson_invar_not_done_2]
+        by (simp add: M_tbd_augment_cong)
+    qed
+  qed
+qed
+
+lemma (in ford_fulkerson_invar_done_1) find_max_matching_psimps:
+  shows "find_max_matching (M_tbd M) = M_tbd M"
+  using done_1
+  by (simp add: find_max_matching_psimps)
+
+lemma (in ford_fulkerson_invar_done_2) find_max_matching_psimps:
+  shows "find_max_matching (M_tbd M) = M_tbd M"
+  using not_done_1 done_2
+  by (simp add: find_max_matching_psimps)
+
+lemma (in ford_fulkerson_invar_not_done_2) find_max_matching_psimps:
+  shows "find_max_matching (M_tbd M) = find_max_matching (M_tbd (augment M (p_tbd G U V s t M)))"
+  using not_done_1 not_done_2
+  by (simp add: find_max_matching_psimps)
+
+lemma (in ford_fulkerson_valid_input_2) loop'_find_max_matching_conv:
+  assumes "ford_fulkerson_invar'' M"
+  shows
+    "M_tbd (loop' G U V s t M) =
+     find_max_match.find_max_matching search_aug_path' (G.E G) (M_tbd M)"
+  using assms
+proof (induct rule: ford_fulkerson_induct[OF assms])
+  case (1 G U V s t M)
+  show ?case
+  proof (cases "done_1 U V M")
+    case True
+    with "1.prems"
+    have "ford_fulkerson_invar_done_1' G U V s t M"
+      by (intro ford_fulkerson_invar_done_1I)
+    thus ?thesis
+      by (simp add: ford_fulkerson_invar_done_1.loop'_psimps ford_fulkerson_invar_done_1.find_max_matching_psimps)
+  next
+    case not_done_1: False
+    show ?thesis
+    proof (cases "done_2 t (m_tbd G U V s t M)")
+      case True
+      with "1.prems" not_done_1
+      have "ford_fulkerson_invar_done_2' G U V s t M"
+        by (intro ford_fulkerson_invar_done_2I_2)
+      thus ?thesis
+        by (simp add: ford_fulkerson_invar_done_2.loop'_psimps ford_fulkerson_invar_done_2.find_max_matching_psimps)
+    next
+      case False
+      with "1.prems" not_done_1
+      have "ford_fulkerson_invar_not_done_2' G U V s t M"
+        by (intro ford_fulkerson_invar_not_done_2I_2)
+      thus ?thesis
+        using not_done_1 False
+        by
+          (auto
+           simp add: ford_fulkerson_invar_not_done_2.loop'_psimps ford_fulkerson_invar_not_done_2.find_max_matching_psimps
+           dest: "1.hyps"(2)
+           intro: ford_fulkerson_invar_not_done_2.ford_fulkerson_invar_augment)
+    qed
+  qed
+qed
+
+lemma (in find_max_match) maximum_matching_find_max_matching:
+  shows "maximum_matching G (find_max_matching {})"
+proof -
+  { fix M
+    assume "graph_matching G M"
+    hence "finite M"
+      using finite_G
+      by (auto intro: finite_subset) }
+  thus ?thesis
+    using find_max_matching_works
+    by (simp add: Berge2.matching_def matching_def)
+qed
+
+theorem (in ford_fulkerson_valid_input_2)
+  shows "maximum_matching (G.E G) (M_tbd (loop' G U V s t M_empty))"
+proof -
+  have "M_tbd (loop' G U V s t M_empty) = find_max_matching {}"
+    using ford_fulkerson_invar_empty
+    by (simp add: loop'_find_max_matching_conv M.map_empty)
+  thus ?thesis
+    using maximum_matching_find_max_matching
+    by presburger
+qed
+
+end
